a few more additions to the generic Rtac file.

theories/Lambda/Rtac.v
@@ -1,4 +1,4 @@
-(** Basics Rtac tactics specialized for the lambda language.
+(** Basic Rtac tactics specialized for the lambda language.
  **)
 Require Import ExtLib.Tactics.
 Require Import MirrorCore.Util.Forwardy.
@@ -24,6 +24,7 @@ Section tactics.
   Let ExprOk_expr : ExprOk Expr_expr := ExprOk_expr.
   Local Existing Instance ExprOk_expr.
 
+  (* Apply Tactics *)
   Definition EAPPLY_depth (depth : nat)
   : Lemma.lemma typ (expr typ func) (expr typ func) ->
     rtac typ (expr typ func) :=
@@ -69,6 +70,72 @@ Section tactics.
     eapply RtacSound_APPLY_depth; assumption.
   Qed.
 
+  (* * Apply tactics with minification *)
+  Definition EAPPLY_m (l : Lemma.lemma typ (expr typ func) (expr typ func))
+  : rtac typ (expr typ func) :=
+    THEN (EAPPLY_depth (S (length l.(Lemma.vars))) l)
+         (@MINIFY _ _ _ _ _).
+
+  Definition APPLY_m (l : Lemma.lemma typ (expr typ func) (expr typ func))
+  : rtac typ (expr typ func) :=
+    THEN (APPLY_depth (S (length l.(Lemma.vars))) l)
+         (@MINIFY _ _ _ _ _).
+
+  Global Instance RtacSound_EAPPLY_m l (RL : ReifiedLemma l)
+  : RtacSound (EAPPLY_m l).
+  Proof.
+    constructor.
+    eapply THEN_sound.
+    - eapply RtacSound_proof. eauto with typeclass_instances.
+    - eapply MINIFY_sound; eauto with typeclass_instances.
+  Qed.
+
+  Global Instance RtacSound_APPLY_m l (RL : ReifiedLemma l)
+  : RtacSound (APPLY_m l).
+  Proof.
+    constructor.
+    eapply THEN_sound.
+    - eapply RtacSound_proof. eauto with typeclass_instances.
+    - eapply MINIFY_sound; eauto with typeclass_instances.
+  Qed.
+
+  (* Assumption Tactics *)
+  Definition EASSUMPTION : rtac typ (expr typ func) :=
+    @EASSUMPTION typ (expr typ func) _ _
+       (fun subst S_subst SU ctx e1 e2 s =>
+          @exprUnify subst typ func _ _ _ S_subst SU 30
+                     (getUVars ctx) (getVars ctx) 0 e1 e2 (typ0 (F:=Prop)) s).
+
+  Global Instance RtacSound_EASSUMPTION : RtacSound EASSUMPTION.
+  Proof.
+    constructor.
+    eapply Assumption.ASSUMPTION_sound.
+    generalize 30.
+    intros.
+    destruct (@exprUnify_sound (ctx_subst ctx) typ func _ _ _ _ _ _ _ _ _ _ n
+               _ _ _ _ _ _ _ nil H H0).
+    split; auto.
+    simpl in *.
+    intros.
+    unfold Ctx.propD, exprD'_typ0 in *.
+    forwardy. inv_all; subst.
+    unfold exprD', tus, tvs in *. simpl in *.
+    destruct (@H2 _ _ sD H3 H4 H5); clear H2.
+    forward_reason.
+    split; eauto.
+    eexists; split; eauto.
+    intros.
+    specialize (H7 _ _ H8).
+    destruct H7.
+    split; auto.
+    specialize (H9 HList.Hnil); simpl in H9.
+    clear - H9.
+    generalize (typ0_cast (F:=Prop)).
+    generalize dependent (typD (typ0 (F:=Prop))).
+    intros; subst. assumption.
+  Defined.
+
+  (* Simplification Tactics *)
   Definition SIMPL (fr : full_reducer typ func) : rtac typ (expr typ func) :=
     SIMPLIFY (fun Tsubst Csubst ctx subst e => fr nil e nil).
 
@@ -106,4 +173,5 @@ Section tactics.
       intros; subst.
       rewrite H4. assumption.
   Qed.
+
 End tactics.
